src/Parsers/ParserFromParserADT.v
@@ -53,8 +53,10 @@ Section parser.
       (adt_based_StringLike_lite splitter_impl)
       (ParserImplementation.parser_data (adt_based_splitter splitter_impl))
       (fun it its str => msplits splitter_impl (it, its) str)
+      (fun prods str => mrules splitter_impl prods str)
     := { proj := @proj1_sig _ _ }.
   Proof.
+    reflexivity.
     reflexivity.
     reflexivity.
     reflexivity.
@@ -63,20 +65,24 @@ Section parser.
   Defined.
 
   Context {constT varT}
-          {strC : @BooleanRecognizerOptimized.str_carrier
+          {strC : @BooleanRecognizerOptimized.str_carrier_data
                     Ascii.ascii
                     (adt_based_StringLike_lite splitter_impl)
-                    constT varT}.
+                    constT varT}
+          {strCH : @BooleanRecognizerOptimized.str_carrier_ok
+                     _ _ _ _ strC}.
 
-  Definition parser : Parser G string_stringlike.
+  Definition parser' : Parser G string_stringlike.
   Proof.
-    refine (@parser ls (adt_based_splitter splitter_impl)
-                    (adt_based_StringLike_lite splitter_impl)
-                    _
-                    adtProj new_string_of_string
-                    (fun rep str => AbsR (projT2 splitter_impl) str (` rep))
-                    (@new_string_of_base_string_R) _ _
-                    _ _ strC);
+    refine (@ParserImplementationOptimized.parser'
+              ls (adt_based_splitter splitter_impl)
+              (adt_based_StringLike_lite splitter_impl)
+              _
+              _
+              adtProj new_string_of_string
+              (fun rep str => AbsR (projT2 splitter_impl) str (` rep))
+              (@new_string_of_base_string_R) _ _
+              _ _ strC _);
     abstract (
         split;
         first [ (intros ????);
@@ -89,6 +95,102 @@ Section parser.
               | intros; refine (mdrop_R _ _); assumption ]
       ).
   Defined.
+
+  Local Arguments new_string_of_base_string : simpl never.
+  Local Arguments BooleanRecognizerOptimized.to_string / .
+  Local Arguments BooleanRecognizerOptimized.of_string_var / .
+  Local Arguments BooleanRecognizerOptimized.of_string_const / .
+  Local Arguments mlength : simpl never.
+  Local Arguments mrules : simpl never.
+  Local Arguments msplits : simpl never.
+  Local Arguments mdrop : simpl never.
+  Local Arguments mtake : simpl never.
+  Local Arguments mis_char : simpl never.
+  Local Arguments cMethods : simpl never.
+  Local Arguments cConstructors : simpl never.
+  Local Arguments BooleanRecognizer.parse_production' / .
+  Local Arguments option_rect / .
+  Local Arguments option_map / .
+  Local Arguments BooleanRecognizer.parse_item' / .
+  Local Arguments RDPList.rdp_list_is_valid_nonterminal / .
+  Local Arguments StringBound.indexb / .
+  Local Arguments StringBound.bindex / .
+  Local Arguments list_to_grammar / .
+  Local Arguments List.hd / .
+  Local Arguments projT1 / .
+  Local Arguments projT2 / .
+  Local Arguments cRep / .
+
+  (*Local Arguments pcMethods / .
+  Local Arguments pcConstructors / .
+  Local Arguments List.nth_error / .
+  Local Arguments List.map / .
+  Local Arguments List.fold_right / .
+  Local Arguments List.fold_left / .
+  Local Arguments Datatypes.length / .
+  Local Arguments List.filter / .
+*)
+
+  Local Ltac pre_do_unfold_0 term tac :=
+    idtac;
+    let term' := (match True with
+                    | _ => eval cbv delta [term] in term
+                    | _ => term
+                  end) in
+    let term'' := (eval cbv beta iota zeta delta [cConstructors pcConstructors cMethods pcMethods fst snd projT1 projT2 List.map List.filter List.nth_error Datatypes.length List.fold_right List.fold_left] in term') in
+    tac term''.
+
+  Local Ltac do_unfold_0_in term impl :=
+    idtac;
+    pre_do_unfold_0 term ltac:(fun term'' =>
+                                 progress change term with term'' in impl);
+    cbv beta in impl.
+
+  Local Ltac do_unfold_0 term :=
+    idtac;
+    pre_do_unfold_0 term ltac:(fun term'' => progress change term with term'');
+    cbv beta.
+
+  Definition parser'' : Parser G string_stringlike.
+  Proof.
+    cut { impl : _ | has_parse parser' = impl }.
+    { intros [impl H].
+      exists impl;
+        abstract (
+            subst;
+            apply parser'
+          ). }
+    { simpl.
+      do_unfold_0 mis_char.
+      do_unfold_0 (Datatypes.length (List.map fst ls)).
+      do_unfold_0 (List.map fst ls).
+      do_unfold_0 mtake.
+      do_unfold_0 msplits.
+      do_unfold_0 mlength.
+      do_unfold_0 mrules.
+      do_unfold_0 new_string_of_base_string.
+      unfold List.map, List.fold_right, List.fold_left, List.nth_error, List.filter.
+      eexists.
+      exact eq_refl. }
+  Defined.
+
+  Definition parser''' : Parser G string_stringlike.
+  Proof.
+    exists (has_parse parser'');
+    abstract apply parser''.
+  Defined.
+
+  Definition parser'''' : Parser G string_stringlike.
+  Proof.
+    let impl := (eval cbv beta iota zeta delta [has_parse parser'' parser'''] in (has_parse parser''')) in
+    (exists impl).
+    { exact (has_parse_sound parser'''). }
+    { exact (has_parse_complete parser'''). }
+  Defined.
+
+  Definition parser : Parser G string_stringlike
+    := Eval cbv delta [parser''''] in parser''''.
+
 End parser.
 
-Global Arguments parser {ls} splitter_impl {constT varT strC}.
+Global Arguments parser {ls} splitter_impl {constT varT strC strCH}.
