src/Parsers/ParserInterface.v
@@ -34,16 +34,35 @@ Section interface.
               -> Forall_parse_of_production (fun _ nt => List.In nt (Valid_nonterminals G)) pits
               -> List.In n splits.
 
+  (** A list of rules is complete if it contains every index of the
+      actual rules that yields a parse tree for that string. *)
+  Definition rules_list_is_complete `{HSL : StringLike Char} (str : String) (nt : String.string)
+             (rules : list nat)
+  : Prop
+    := List.In nt (Valid_nonterminals G)
+       -> forall n its,
+            List.nth_error (Lookup G nt) n = Some its
+            -> forall (p : parse_of_production G str its),
+                 Forall_parse_of_production (fun _ nt => List.In nt (Valid_nonterminals G)) p
+                 -> List.In n rules.
+
   Record Splitter :=
     {
       string_type :> StringLike Char;
       splits_for : String -> item Char -> production Char -> list nat;
       (** give a list of indices for splitting a given string *)
 
+      rules_for : String -> productions Char -> list nat;
+      (** give a list of indices for the rules of a given list of productions for a given string *)
+
       string_type_properties :> StringLikeProperties Char;
       splits_for_complete : forall str it its,
-                              split_list_is_complete str it its (splits_for str it its)
+                              split_list_is_complete str it its (splits_for str it its);
       (** [splits_for] must contain all valid indices for splitting *)
+
+      rules_for_complete : forall str nt,
+                              rules_list_is_complete str nt (rules_for str (Lookup G nt))
+      (** [rules_for] must contain all valid indices for productions *)
     }.
 
   Global Existing Instance string_type.
@@ -56,7 +75,10 @@ Section interface.
 
       has_parse_sound : forall str,
                           has_parse str = true
-                          -> parse_of_item G str (NonTerminal (Start_symbol G));
+                          -> { p : parse_of_item G str (NonTerminal (Start_symbol G))
+                                   & Forall_parse_of_item
+                                       (fun _ nt => List.In nt (Valid_nonterminals G))
+                                       p };
 
       has_parse_complete : forall str (p : parse_of_item G str (NonTerminal (Start_symbol G))),
                              Forall_parse_of_item
