src/Parsers/Refinement/IndexedAndAtMostOneNonTerminalReflective.v
@@ -1,6 +1,7 @@
 (** First step of a splitter refinement; indexed representation, and handle all rules with at most one nonterminal; leave a reflective goal *)
 Require Import Coq.Strings.String Coq.Arith.Lt Coq.Lists.List.
 Require Import Coq.Numbers.Natural.Peano.NPeano.
+Require Import Fiat.Common.List.Operations.
 Require Import Fiat.Parsers.StringLike.Core.
 Require Import Fiat.Parsers.ParserInterface.
 Require Import Fiat.Parsers.ParserADTSpecification.
@@ -8,6 +9,8 @@ Require Import Fiat.Parsers.StringLike.Properties.
 Require Import Fiat.Parsers.StringLike.String.
 Require Import Fiat.Parsers.ContextFreeGrammarEquality.
 Require Import Fiat.Parsers.ContextFreeGrammarProperties.
+Require Import Fiat.Parsers.ContextFreeGrammarPropertiesRDPList.
+Require Import Fiat.Parsers.Refinement.DisjointLemmas.
 Require Import Fiat.Parsers.Refinement.FixedLengthLemmas.
 Require Import ADTNotation.BuildADT ADTNotation.BuildADTSig.
 Require Import ADT.ComputationalADT.
@@ -223,6 +226,106 @@ Proof.
     specialize (H (p::ps)); eauto. }
 Qed.
 
+Fixpoint all_disjoint {A} (beq : A -> A -> bool) (ls : list (list A))
+  := match ls with
+       | nil => true
+       | x::xs => andb
+                    (fold_right
+                       andb
+                       true
+                       (map
+                          (disjoint beq x)
+                          xs))
+                    (all_disjoint beq xs)
+     end.
+
+
+Lemma all_disjoint_fold_computes_in {T} {ls : list (list T)} {v1 v0} {a k n}
+      (beq : T -> T -> bool) (bl : forall x y, beq x y -> x = y) (lb : forall x y, x = y -> beq x y)
+      (Hdisjoint : all_disjoint beq ls)
+      (H_comp : fold_right
+                  (fun (n_chars : nat * list T)
+                       (else_case' : Comp (list nat)) =>
+                     If list_bin beq a (snd n_chars) Then
+                        ret [fst n_chars] Else else_case') (ret v0)
+                  (enumerate ls k) ↝ v1)
+: (fold_right orb false (map (list_bin beq a) ls) = false
+   /\ v1 = v0)
+  \/ (List.In (k + n) v1
+      <-> (exists its, nth_error ls n = Some its
+                       /\ list_bin beq a its)).
+Proof.
+  destruct (fold_right orb false (map (list_bin beq a) ls)) eqn:H; [ right | left; split; [ reflexivity | ] ].
+  { generalize dependent k; revert n.
+    induction ls; simpl in *; try discriminate; [].
+    apply Bool.andb_true_iff in Hdisjoint.
+    destruct Hdisjoint as [Hdisjoint0 Hdisjoint].
+    specialize_by assumption.
+    apply Bool.orb_true_iff in H.
+    destruct H as [H|H]; specialize_by assumption.
+    { rewrite H; simpl.
+      intros; computes_to_inv; subst; simpl.
+      destruct n; split; intros; try omega; simpl.
+      { eexists; split; [ reflexivity | eassumption ]. }
+      { destruct_head ex.
+        destruct_head and.
+        exfalso; eapply some_disjoint; eassumption. } }
+    { destruct (list_bin beq a a0) eqn:H'; simpl in *; try discriminate.
+      { intros [|n]; intros; computes_to_inv; subst; simpl.
+        { split; intuition; eauto. }
+        { split; intuition.
+          destruct_head ex.
+          destruct_head and.
+          exfalso; eapply some_disjoint; eassumption. } }
+      { intros [|n]; intros; computes_to_inv; subst; simpl.
+        { split; intro H''.
+          { exfalso.
+            clear -H'' H_comp H.
+            assert (k + 0 < S k) by omega.
+            generalize dependent (k + 0).
+            generalize dependent (S k).
+            induction ls; simpl in *; computes_to_inv; subst; try discriminate.
+            repeat match goal with
+                     | [ H : orb _ _ = true |- _ ] => apply Bool.orb_true_iff in H
+                     | [ H : ?x = true |- _ ] => rewrite H
+                     | _ => progress simpl in *
+                     | _ => progress destruct_head or
+                     | _ => progress specialize_by assumption
+                     | _ => progress intros
+                     | _ => progress computes_to_inv
+                     | _ => progress subst
+                     | _ => omega
+                     | [ H : context[If ?e Then _ Else _] |- _ ] => destruct e eqn:?
+                     | [ H : forall n, computes_to (fold_right _ _ _) _ -> _, H' : computes_to (fold_right _ _ _) _ |- _ ]
+                       => specialize (H _ H')
+                     | _ => solve [ eauto ]
+                   end. }
+          { destruct_head ex.
+            destruct_head and.
+            repeat match goal with
+                     | _ => progress unfold value in *
+                     | [ H : Some _ = Some _ |- _ ]
+                       => (inversion H; clear H)
+                     | _ => progress subst
+                     | _ => discriminate
+                     | _ => congruence
+                   end.  } }
+        { specialize (IHls n (S k)).
+          repeat match goal with
+                   | [ H : context[_ + S _] |- _ ] => rewrite <- plus_n_Sm in H
+                   | [ |- context[_ + S _] ] => rewrite <- plus_n_Sm
+                   | [ H : context[_ + 0] |- _ ] => rewrite <- plus_n_O in H
+                   | _ => auto
+                 end. } } } }
+  { generalize dependent k; induction ls; simpl in *; intros; computes_to_inv; subst; trivial.
+    edestruct (@list_bin); simpl in *; try discriminate.
+    apply Bool.andb_true_iff in Hdisjoint.
+    destruct Hdisjoint as [Hdisjoint0 Hdisjoint].
+    specialize_by assumption.
+    specialize (IHls (S k)).
+    specialize_by assumption; trivial. }
+Qed.
+
 Section helpers.
   Section generic.
     Context {Char : Type}.
@@ -287,165 +390,345 @@ Section IndexedImpl.
     (min (String.length (fst s) - fst (snd s)) (snd (snd s)))
       (only parsing).
   Local Notation iget n s :=
-    (get n (string_of_indexed s))
+    (StringLike.get n (string_of_indexed s))
       (only parsing).
 
-  Definition expanded_fallback_list'
-             (P : String -> item Ascii.ascii -> production Ascii.ascii -> item Ascii.ascii -> production Ascii.ascii -> list nat -> Prop)
-             (s : T)
-             (it : item Ascii.ascii) (its : production Ascii.ascii)
-             (dummy : list nat)
-  : Comp (T * list nat)
-    := (ls <- (forall_reachable_productions
+  Section splits.
+    Definition expanded_fallback_list'
+               (P : String -> item Ascii.ascii -> production Ascii.ascii -> item Ascii.ascii -> production Ascii.ascii -> list nat -> Prop)
+               (s : T)
+               (it : item Ascii.ascii) (its : production Ascii.ascii)
+               (dummy : list nat)
+    : Comp (T * list nat)
+      := (ls <- (forall_reachable_productions
+                   G
+                   (fun p else_case
+                    => If production_beq ascii_beq p (it::its)
+                          Then (match p return Comp (list nat) with
+                                  | nil => ret dummy
+                                  | _::nil => ret [ilength s]
+                                  | (Terminal _):: _ :: _ => ret [1]
+                                  | (NonTerminal nt):: p'
+                                    => If has_only_terminals p'
+                                          Then
+                                          ret [(ilength s - Datatypes.length p')%natr]
+                                          Else
+                                          (option_rect
+                                             (fun _ => Comp (list nat))
+                                             (fun (n : nat) => ret [n])
+                                             { splits : list nat
+                                             | P
+                                                 (string_of_indexed s)
+                                                 (NonTerminal nt)
+                                                 p'
+                                                 it
+                                                 its
+                                                 splits }%comp
+                                             (length_of_any G nt))
+                                end)
+                          Else else_case)
+                   (ret dummy));
+          ret (s, ls))%comp.
+
+    Global Arguments expanded_fallback_list' / .
+
+    Definition expanded_fallback_list
+      := expanded_fallback_list' (fun str it its _ _ => split_list_is_complete G str it its).
+    Definition split_list_is_complete_case
+               str it its it' its' splits
+      := forall n,
+           n <= length str
+           -> production_is_reachable G (it'::its')
+           -> forall (pit : parse_of_item G (take n str) it)
+                     (pits : parse_of_production G (drop n str) its),
+                Forall_parse_of_item (fun _ nt => List.In nt (Valid_nonterminals G)) pit
+                -> Forall_parse_of_production (fun _ nt => List.In nt (Valid_nonterminals G)) pits
+                -> List.In n splits.
+    Definition expanded_fallback_list_case
+      := expanded_fallback_list' split_list_is_complete_case.
+
+    Definition split_list_is_complete_alt
+      := (fun str it its splits
+          => forall n,
+               n <= length str
+               -> forall (pit : parse_of_item G (take n str) it)
+                         (pits : parse_of_production G (drop n str) its),
+                    Forall_parse_of_item (fun _ nt => List.In nt (Valid_nonterminals G)) pit
+                    -> Forall_parse_of_production (fun _ nt => List.In nt (Valid_nonterminals G)) pits
+                    -> List.In n splits).
+
+    Definition expanded_fallback_list_alt
+      := expanded_fallback_list' (fun str it its _ _ => split_list_is_complete_alt str it its).
+
+    Global Arguments expanded_fallback_list / .
+    Global Arguments expanded_fallback_list_alt / .
+    Global Arguments expanded_fallback_list_case / .
+
+    Lemma expanded_fallback_list'_ext'
+          (P1 P2 : String -> item Ascii.ascii -> production Ascii.ascii -> item Ascii.ascii -> production Ascii.ascii -> list nat -> Prop)
+          str it its dummy
+          (H : forall splits,
+                 P2 (string_of_indexed str) it its it its splits
+                 -> P1 (string_of_indexed str) it its it its splits)
+    : refine (expanded_fallback_list' P1 str it its dummy)
+             (expanded_fallback_list' P2 str it its dummy).
+    Proof.
+      simpl.
+      repeat intro; computes_to_inv; subst.
+      eapply BindComputes; [ | apply ReturnComputes ].
+      unfold forall_reachable_productions in *.
+      induction ((flatten
+                    (flatten
+                       (map (fun nt : string => map tails (G nt)) (Valid_nonterminals G)))))
+        as [ | x xs IHG ]; simpl in *; trivial; [].
+      match goal with
+        | [ |- context[production_beq ?x ?y ?z] ]
+          => destruct (production_beq x y z) eqn:Heqb
+      end;
+        simpl in *; eauto; [].
+      apply (production_bl (@ascii_bl)) in Heqb;
+        instantiate; subst; unfold option_rect, If_Then_Else in *;
+        repeat match goal with
+                 | _ => assumption
+                 | _ => solve [ eauto ]
+                 | [ |- context[match ?e with _ => _ end] ]
+                   => atomic e; destruct e
+                 | [ |- context[match ?e with _ => _ end] ]
+                   => destruct e eqn:?
+                 | _ => progress simpl in *
+                 | _ => progress computes_to_inv
+                 | [ |- computes_to (Pick _) _ ] => apply PickComputes
+               end.
+    Qed.
+
+    Lemma expanded_fallback_list'_ext''
+          (P1 P2 : String -> item Ascii.ascii -> production Ascii.ascii -> item Ascii.ascii -> production Ascii.ascii -> list nat -> Prop)
+          str it its dummy
+          (H : forall_reachable_productions
                  G
-                 (fun p else_case
-                  => If production_beq ascii_beq p (it::its)
-                     Then (match p return Comp (list nat) with
-                             | nil => ret dummy
-                             | _::nil => ret [ilength s]
-                             | (Terminal _):: _ :: _ => ret [1]
-                             | (NonTerminal nt):: p'
-                               => If has_only_terminals p'
-                                  Then
-                                    ret [(ilength s - Datatypes.length p')%natr]
-                                  Else
-                                  (option_rect
-                                     (fun _ => Comp (list nat))
-                                     (fun (n : nat) => ret [n])
-                                     { splits : list nat
-                                     | P
-                                         (string_of_indexed s)
-                                         (NonTerminal nt)
-                                         p'
-                                         it
-                                         its
-                                         splits }%comp
-                                     (length_of_any G nt))
-                           end)
-                     Else else_case)
-                 (ret dummy));
-        ret (s, ls))%comp.
+                 (fun p H
+                  => match p with
+                       | nil => True
+                       | it'::its'
+                         => forall splits,
+                              P2 (string_of_indexed str) it' its' it' its' splits
+                              -> P1 (string_of_indexed str) it' its' it' its' splits
+                     end /\ H)
+                 True)
+    : refine (expanded_fallback_list' P1 str it its dummy)
+             (expanded_fallback_list' P2 str it its dummy).
+    Proof.
+      simpl.
+      repeat intro; computes_to_inv; subst.
+      eapply BindComputes; [ | apply ReturnComputes ].
+      unfold forall_reachable_productions in *.
+      induction ((flatten
+                    (flatten
+                       (map (fun nt : string => map tails (G nt)) (Valid_nonterminals G)))))
+        as [ | x xs IHG ]; simpl in *; trivial; [].
+      progress destruct_head and.
+      match goal with
+        | [ |- context[production_beq ?x ?y ?z] ]
+          => destruct (production_beq x y z) eqn:Heqb
+      end;
+        simpl in *; eauto; [].
+      apply (production_bl (@ascii_bl)) in Heqb;
+        instantiate; subst; unfold option_rect, If_Then_Else in *;
+        repeat match goal with
+                 | _ => assumption
+                 | _ => solve [ eauto ]
+                 | [ |- context[match ?e with _ => _ end] ]
+                   => atomic e; destruct e
+                 | [ |- context[match ?e with _ => _ end] ]
+                   => destruct e eqn:?
+                 | _ => progress simpl in *
+                 | _ => progress computes_to_inv
+                 | [ |- computes_to (Pick _) _ ] => apply PickComputes
+               end.
+    Qed.
+  End splits.
 
-  Global Arguments expanded_fallback_list' / .
+  Section rules.
+    Definition expanded_fallback_list_rules'
+               (P : String -> productions Ascii.ascii -> productions Ascii.ascii -> list nat -> Prop)
+               (s : T)
+               (prods : productions Ascii.ascii)
+               (dummy : list nat)
+    : Comp (T * list nat)
+      := (ls <- (fold_right
+                   (fun p else_case
+                    => If productions_beq ascii_beq p prods
+                          Then (match p return Comp (list nat) with
+                                  | nil => ret [0]
+                                  | _::nil => ret [0]
+                                  | p'
+                                    => option_rect
+                                         (fun _ => Comp (list nat))
+                                         (fun ch
+                                          => let possible_chars
+                                                 := map
+                                                      (possible_first_terminals_of_production G : _ -> list _)
+                                                      p' in
+                                             If all_disjoint ascii_beq possible_chars
+                                             Then (fold_right
+                                                     (fun n_chars else_case'
+                                                      => If list_bin ascii_beq ch (snd n_chars)
+                                                            Then ret [fst n_chars]
+                                                            Else else_case')
+                                                     (ret dummy)
+                                                     (enumerate possible_chars 0))
+                                             Else { rules : list nat
+                                                  | P
+                                                      (string_of_indexed s)
+                                                      p'
+                                                      prods
+                                                      rules }%comp)
+                                         (ret (List.map
+                                                 fst
+                                                 (List.filter
+                                                    (fun nits
+                                                     => might_be_empty (possible_first_terminals_of_production G (snd nits)))
+                                                    (enumerate p' 0))))
+                                         (iget 0 s)
+                                end)
+                          Else else_case)
+                   (ret dummy)
+                   (map
+                      (Lookup G)
+                      (Valid_nonterminals G)));
+          ret (s, ls))%comp.
 
-  Definition expanded_fallback_list
-    := expanded_fallback_list' (fun str it its _ _ => split_list_is_complete G str it its).
-  Definition split_list_is_complete_case
-             str it its it' its' splits
-    := forall n,
-         n <= length str
-         -> production_is_reachable G (it'::its')
-         -> forall (pit : parse_of_item G (take n str) it)
-                   (pits : parse_of_production G (drop n str) its),
-              Forall_parse_of_item (fun _ nt => List.In nt (Valid_nonterminals G)) pit
-              -> Forall_parse_of_production (fun _ nt => List.In nt (Valid_nonterminals G)) pits
-              -> List.In n splits.
-  Definition expanded_fallback_list_case
-    := expanded_fallback_list' split_list_is_complete_case.
+    Global Arguments expanded_fallback_list_rules' / .
 
-  Definition split_list_is_complete_alt
-    := (fun str it its splits
-        => forall n,
-             n <= length str
-             -> forall (pit : parse_of_item G (take n str) it)
-                       (pits : parse_of_production G (drop n str) its),
-                  Forall_parse_of_item (fun _ nt => List.In nt (Valid_nonterminals G)) pit
-                  -> Forall_parse_of_production (fun _ nt => List.In nt (Valid_nonterminals G)) pits
-                  -> List.In n splits).
+    Definition expanded_fallback_list_rules
+      := expanded_fallback_list_rules' (fun str prods _ ls => forall nt, Lookup G nt = prods -> rules_list_is_complete G str nt ls).
+    Definition rules_list_is_complete_case
+               str (prods prods' : productions Ascii.ascii) rules
+      := forall nt,
+           Lookup G nt = prods
+           -> rules_list_is_complete G str nt rules.
+    Definition expanded_fallback_list_rules_case
+      := expanded_fallback_list_rules' rules_list_is_complete_case.
 
-  Definition expanded_fallback_list_alt
-    := expanded_fallback_list' (fun str it its _ _ => split_list_is_complete_alt str it its).
+    (*Definition split_list_is_complete_alt
+      := (fun str it its splits
+          => forall n,
+               n <= length str
+               -> forall (pit : parse_of_item G (take n str) it)
+                         (pits : parse_of_production G (drop n str) its),
+                    Forall_parse_of_item (fun _ nt => List.In nt (Valid_nonterminals G)) pit
+                    -> Forall_parse_of_production (fun _ nt => List.In nt (Valid_nonterminals G)) pits
+                    -> List.In n splits).
 
-  Global Arguments expanded_fallback_list / .
-  Global Arguments expanded_fallback_list_alt / .
-  Global Arguments expanded_fallback_list_case / .
+(*List.In nt (Valid_nonterminals G)
+       -> forall n its,
+            List.nth_error (Lookup G nt) n = Some its
+            -> forall (p : parse_of_production G str its),
+                 Forall_parse_of_production (fun _ nt => List.In nt (Valid_nonterminals G)) p
+                 -> List.In n rules.*)
 
-  Lemma expanded_fallback_list'_ext'
-        (P1 P2 : String -> item Ascii.ascii -> production Ascii.ascii -> item Ascii.ascii -> production Ascii.ascii -> list nat -> Prop)
-        str it its dummy
-        (H : forall splits,
-               P2 (string_of_indexed str) it its it its splits
-               -> P1 (string_of_indexed str) it its it its splits)
-  : refine (expanded_fallback_list' P1 str it its dummy)
-           (expanded_fallback_list' P2 str it its dummy).
-  Proof.
-    simpl.
-    repeat intro; computes_to_inv; subst.
-    eapply BindComputes; [ | apply ReturnComputes ].
-    unfold forall_reachable_productions in *.
-    induction ((flatten
-                  (flatten
-                     (map (fun nt : string => map tails (G nt)) (Valid_nonterminals G)))))
-      as [ | x xs IHG ]; simpl in *; trivial; [].
-    match goal with
-      | [ |- context[production_beq ?x ?y ?z] ]
-        => destruct (production_beq x y z) eqn:Heqb
-    end;
-      simpl in *; eauto; [].
-    apply (production_bl (@ascii_bl)) in Heqb;
-      instantiate; subst; unfold option_rect, If_Then_Else in *;
+    Definition expanded_fallback_list_alt
+      := expanded_fallback_list' (fun str prods _ _ => split_list_is_complete_alt str it its).*)
+
+    Global Arguments expanded_fallback_list_rules / .
+    (*Global Arguments expanded_fallback_list_alt / .*)
+    Global Arguments expanded_fallback_list_rules_case / .
+
+    Lemma expanded_fallback_list_rules'_ext'
+          (P1 P2 : String -> productions Ascii.ascii -> productions Ascii.ascii -> list nat -> Prop)
+          str prods dummy
+          (H : forall rules,
+                 P2 (string_of_indexed str) prods prods rules
+                 -> P1 (string_of_indexed str) prods prods rules)
+    : refine (expanded_fallback_list_rules' P1 str prods dummy)
+             (expanded_fallback_list_rules' P2 str prods dummy).
+    Proof.
+      simpl.
+      repeat intro; computes_to_inv; subst.
+      eapply BindComputes; [ | apply ReturnComputes ].
+      induction (Valid_nonterminals G)
+        as [ | x xs IHG ]; simpl in *; trivial; [].
+      match goal with
+        | [ |- context[productions_beq ?x ?y ?z] ]
+          => destruct (productions_beq x y z) eqn:Heqb
+      end;
+        simpl in *; [ clear IHG | solve [ eauto ] ].
+      apply (productions_bl (@ascii_bl)) in Heqb;
+        instantiate; subst.
+      destruct (Lookup G x) as [|Gx [|Gx' Gxs]]; [ assumption | assumption | ].
+      match goal with
+        | [ |- context[option_rect _ _ _ ?x] ]
+          => destruct x eqn:?; [ | assumption ]
+      end; unfold option_rect in *.
+      match goal with
+        | [ |- context[fold_right _ _ ?ls] ] => generalize dependent ls
+      end.
+      intro ls.
+      match type of H with
+        | forall rules, ?P2 rules -> ?P1 rules
+          => generalize dependent P2;
+            generalize P1
+      end.
+      intros ???.
+      generalize (Gx :: Gx' :: Gxs); intro.
+      induction ls;
       repeat match goal with
-               | _ => assumption
-               | _ => solve [ eauto ]
-               | [ |- context[match ?e with _ => _ end] ]
-                 => atomic e; destruct e
-               | [ |- context[match ?e with _ => _ end] ]
-                 => destruct e eqn:?
                | _ => progress simpl in *
-               | _ => progress computes_to_inv
-               | [ |- computes_to (Pick _) _ ] => apply PickComputes
+               | [ |- context[If ?b Then _ Else _] ] => destruct b eqn:?
+               | _ => intros; assumption
+               | _ => solve [ auto ]
              end.
-  Qed.
+    Qed.
 
-  Lemma expanded_fallback_list'_ext''
-        (P1 P2 : String -> item Ascii.ascii -> production Ascii.ascii -> item Ascii.ascii -> production Ascii.ascii -> list nat -> Prop)
-        str it its dummy
-        (H : forall_reachable_productions
-               G
-               (fun p H
-                => match p with
-                     | nil => True
-                     | it'::its'
-                       => forall splits,
-                            P2 (string_of_indexed str) it' its' it' its' splits
-                            -> P1 (string_of_indexed str) it' its' it' its' splits
-                   end /\ H)
-               True)
-  : refine (expanded_fallback_list' P1 str it its dummy)
-           (expanded_fallback_list' P2 str it its dummy).
-  Proof.
-    simpl.
-    repeat intro; computes_to_inv; subst.
-    eapply BindComputes; [ | apply ReturnComputes ].
-    unfold forall_reachable_productions in *.
-    induction ((flatten
-                  (flatten
-                     (map (fun nt : string => map tails (G nt)) (Valid_nonterminals G)))))
-      as [ | x xs IHG ]; simpl in *; trivial; [].
-    progress destruct_head and.
-    match goal with
-      | [ |- context[production_beq ?x ?y ?z] ]
-        => destruct (production_beq x y z) eqn:Heqb
-    end;
-      simpl in *; eauto; [].
-    apply (production_bl (@ascii_bl)) in Heqb;
-      instantiate; subst; unfold option_rect, If_Then_Else in *;
-      repeat match goal with
-               | _ => assumption
-               | _ => solve [ eauto ]
-               | [ |- context[match ?e with _ => _ end] ]
-                 => atomic e; destruct e
-               | [ |- context[match ?e with _ => _ end] ]
-                 => destruct e eqn:?
-               | _ => progress simpl in *
-               | _ => progress computes_to_inv
-               | [ |- computes_to (Pick _) _ ] => apply PickComputes
-             end.
-  Qed.
+    (*Lemma expanded_fallback_list_rules'_ext''
+          (P1 P2 : String -> productions Ascii.ascii -> productions Ascii.ascii -> list nat -> Prop)
+          str prods dummy
+          (H : fold_right
+                 (fun p H
+                  => forall rules,
+                       P2 (string_of_indexed str) p p splits
+                       -> P1 (string_of_indexed str) p p splits
+                     end /\ H)
+                 True
+                 (map (Lookup G) (Valid_nonterminals G)))
+    : refine (expanded_fallback_list' P1 str it its dummy)
+             (expanded_fallback_list' P2 str it its dummy).
+    Proof.
+      simpl.
+      repeat intro; computes_to_inv; subst.
+      eapply BindComputes; [ | apply ReturnComputes ].
+      unfold forall_reachable_productions in *.
+      induction ((flatten
+                    (flatten
+                       (map (fun nt : string => map tails (G nt)) (Valid_nonterminals G)))))
+        as [ | x xs IHG ]; simpl in *; trivial; [].
+      progress destruct_head and.
+      match goal with
+        | [ |- context[production_beq ?x ?y ?z] ]
+          => destruct (production_beq x y z) eqn:Heqb
+      end;
+        simpl in *; eauto; [].
+      apply (production_bl (@ascii_bl)) in Heqb;
+        instantiate; subst; unfold option_rect, If_Then_Else in *;
+        repeat match goal with
+                 | _ => assumption
+                 | _ => solve [ eauto ]
+                 | [ |- context[match ?e with _ => _ end] ]
+                   => atomic e; destruct e
+                 | [ |- context[match ?e with _ => _ end] ]
+                   => destruct e eqn:?
+                 | _ => progress simpl in *
+                 | _ => progress computes_to_inv
+                 | [ |- computes_to (Pick _) _ ] => apply PickComputes
+               end.
+    Qed.*)
+  End rules.
+
+
 
   (** Reference implementation of a [String] that can be split; has a [string], and a start index, and a length *)
 
-  Definition rindexed_spec' P : ADT (string_rep Ascii.ascii) := ADTRep T {
+  Definition rindexed_spec' P Q : ADT (string_rep Ascii.ascii) := ADTRep T {
     Def Constructor "new"(s : String.string) : rep :=
       ret (s, (0, String.length s)),
 
@@ -469,15 +752,24 @@ Section IndexedImpl.
 
     Def Method "splits"(s : rep, p : item Ascii.ascii * production Ascii.ascii) : list nat :=
       dummy <- { ls : list nat | True };
-      expanded_fallback_list' P s (fst p) (snd p) dummy
+      expanded_fallback_list' P s (fst p) (snd p) dummy,
+
+    Def Method "rules"(s : rep, p : productions Ascii.ascii) : list nat :=
+      dummy <- { ls : list nat | True };
+      expanded_fallback_list_rules' Q s p dummy
+
   }.
 
   Definition rindexed_spec : ADT (string_rep Ascii.ascii)
-    := rindexed_spec' (fun str it its _ _ => split_list_is_complete G str it its).
+    := rindexed_spec'
+         (fun str it its _ _ => split_list_is_complete G str it its)
+         (fun str prods _ rules =>
+            forall nt, Lookup G nt = prods -> rules_list_is_complete G str nt rules).
 
   Local Ltac fin :=
     repeat match goal with
              | _ => progress unfold split_list_is_complete
+             | _ => progress unfold rules_list_is_complete
              | _ => progress simpl in *
              | _ => progress computes_to_inv
              | _ => progress subst
@@ -571,9 +863,11 @@ Section IndexedImpl.
 
   Local Arguments expanded_fallback_list' : simpl never.
   Local Opaque expanded_fallback_list'.
+  Local Arguments expanded_fallback_list_rules' : simpl never.
+  Local Opaque expanded_fallback_list_rules'.
 
   Lemma FirstStep_helper_1
-  : refineADT (rindexed_spec' split_list_is_complete_case) rindexed_spec.
+  : refineADT (rindexed_spec' split_list_is_complete_case rules_list_is_complete_case) rindexed_spec.
   Proof.
     econstructor 1; try instantiate (1 := eq);
     eapply Iterate_Ensemble_BoundedIndex_equiv;
@@ -581,23 +875,30 @@ Section IndexedImpl.
     simpl; intros; repeat split;
     try solve [ intuition; intros; try simplify with monad laws;
                 repeat intro; computes_to_inv; subst; simpl;
-                fin ].
-    intros; subst.
-    setoid_rewrite refineEquiv_pick_eq'.
-    simplify with monad laws.
-    assert (H' : forall A B (x : A * B), (fst x, snd x) = x) by (intros; destruct x; reflexivity).
-    setoid_rewrite H'.
-    simplify with monad laws.
-    eapply refine_under_bind_helper_2; [ | reflexivity ]; instantiate; simpl.
-    intros.
-    etransitivity; [ | eassumption ]; instantiate; clear.
-    apply expanded_fallback_list'_ext'; simpl.
-    exact (fun _ x => x).
+                fin ];
+    intros; subst;
+    setoid_rewrite refineEquiv_pick_eq';
+    simplify with monad laws;
+    assert (H' : forall A B (x : A * B), (fst x, snd x) = x) by (intros; destruct x; reflexivity);
+    setoid_rewrite H';
+    simplify with monad laws;
+    (eapply refine_under_bind_helper_2; [ | reflexivity ]); instantiate; simpl;
+    intros;
+    (etransitivity; [ | eassumption ]); instantiate; clear.
+    { apply expanded_fallback_list'_ext'; simpl.
+      exact (fun _ x => x). }
+    { apply expanded_fallback_list_rules'_ext'; simpl.
+      exact (fun _ x => x). }
   Qed.
 
+  Local Opaque rules_list_is_complete_case.
+  Local Opaque expanded_fallback_list'.
+  Local Opaque expanded_fallback_list_rules'.
+
   Lemma FirstStep_helper_2
-  : refineADT (rindexed_spec' (fun str it its _ _ => split_list_is_complete_alt str it its))
-              (rindexed_spec' split_list_is_complete_case).
+  : refineADT (rindexed_spec' (fun str it its _ _ => split_list_is_complete_alt str it its)
+                              rules_list_is_complete_case)
+              (rindexed_spec' split_list_is_complete_case rules_list_is_complete_case).
   Proof.
     econstructor 1; try instantiate (1 := eq);
     eapply Iterate_Ensemble_BoundedIndex_equiv;
@@ -605,14 +906,14 @@ Section IndexedImpl.
     simpl; intros; repeat split;
     try solve [ intuition; intros; try simplify with monad laws;
                 repeat intro; computes_to_inv; subst; simpl;
-                fin ].
-    intros; subst.
-    Local Opaque expanded_fallback_list'.
-    setoid_rewrite refineEquiv_pick_eq'.
-    simplify with monad laws.
-    assert (H' : forall A B (x : A * B), (fst x, snd x) = x) by (intros; destruct x; reflexivity).
-    setoid_rewrite H'.
-    simplify with monad laws.
+                fin ];
+    intros; subst;
+    setoid_rewrite refineEquiv_pick_eq';
+    simplify with monad laws;
+    assert (H' : forall A B (x : A * B), (fst x, snd x) = x) by (intros; destruct x; reflexivity);
+    setoid_rewrite H';
+    simplify with monad laws;
+    [ | reflexivity ].
     eapply refine_under_bind_helper_2; [ | reflexivity ]; instantiate; simpl.
     intros.
     etransitivity; [ | eassumption ]; instantiate; clear.
@@ -623,13 +924,16 @@ Section IndexedImpl.
   Qed.
 
   Local Transparent expanded_fallback_list'.
+  Local Transparent expanded_fallback_list_rules'.
+  Local Arguments StringLike.get : simpl never.
+  Local Transparent rules_list_is_complete_case.
 
   Lemma FirstStep
   : refineADT (string_spec G) rindexed_spec.
   Proof.
     refine (transitivityT _ _ _ _ FirstStep_helper_1).
     refine (transitivityT _ _ _ _ FirstStep_helper_2).
-    unfold rindexed_spec', expanded_fallback_list', split_list_is_complete_alt.
+    unfold rindexed_spec', expanded_fallback_list', split_list_is_complete_alt, expanded_fallback_list_rules'.
     econstructor 1 with (AbsR := (fun r_o r_n =>
                                     substring (fst (snd r_n)) (snd (snd r_n)) (fst r_n) = r_o));
 
@@ -638,72 +942,272 @@ Section IndexedImpl.
         simpl; intuition; intros; try simplify with monad laws;
         repeat intro; computes_to_inv; subst; simpl;
         fin.
-    intros.
-    match goal with
-      | [ H' : appcontext[forall_reachable_productions], H : production_is_reachable G (?x::?xs) |- _ ]
-        => move H' at top; move H at top; generalize dependent xs; intros xs H H';
-           move H' at top; move H at top; generalize dependent x; intros x H; revert x xs H
-    end.
-    refine (proj2 (@production_is_reachable__forall_reachable_productions' Ascii.ascii G _) _).
-    apply (forall_reachable_productions_helper (@ascii_bl) (@ascii_lb)).
-    unfold forall_reachable_productions.
-    lazymatch goal with
+    { intros.
+      match goal with
+        | [ H' : appcontext[forall_reachable_productions], H : production_is_reachable G (?x::?xs) |- _ ]
+          => move H' at top; move H at top; generalize dependent xs; intros xs H H';
+             move H' at top; move H at top; generalize dependent x; intros x H; revert x xs H
+      end.
+      refine (proj2 (@production_is_reachable__forall_reachable_productions' Ascii.ascii G _) _).
+      apply (forall_reachable_productions_helper (@ascii_bl) (@ascii_lb)).
+      unfold forall_reachable_productions.
+      lazymatch goal with
       | [ |- context[fold_right (fun x y => @?P x /\ y) _ _] ]
         => let H' := fresh in
            pose proof (fold_right_map P and) as H';
              unfold compose in H'; simpl in H';
              rewrite <- H'; clear H'
-    end.
-    generalize (flatten
-                  (flatten
-                     (map (fun nt : string => map tails (G nt))
-                          (Valid_nonterminals G)))).
-    intro ls; induction ls; simpl; trivial; [].
-    { repeat match goal with
-               | [ |- _ /\ _ ] => split
-               | [ |- context[match ?e with _ => _ end] ] => atomic e; destruct e
-               | [ |- context[production_beq _ ?x ?x] ] => rewrite (production_lb (@ascii_lb) eq_refl)
-               | _ => solve [ trivial ]
-             end.
-      { clear IHls; intros; abstract fin. }
-      { clear IHls; intros; abstract fin. }
-      { clear IHls; intros; abstract fin. }
-      { clear IHls; unfold If_Then_Else, option_rect.
-        repeat match goal with
-                 | [ |- context[if has_only_terminals ?e then _ else _] ]
-                   => case_eq (has_only_terminals e)
-                 | [ |- context[match ?e with None => _ | _ => _ end] ]
-                   => case_eq e
-               end;
-          try
-            abstract (
+      end.
+      generalize (flatten
+                    (flatten
+                       (map (fun nt : string => map tails (G nt))
+                            (Valid_nonterminals G)))).
+      intro ls; induction ls; simpl; trivial; [].
+      { repeat match goal with
+                 | [ |- _ /\ _ ] => split
+                 | [ |- context[match ?e with _ => _ end] ] => atomic e; destruct e
+                 | [ |- context[production_beq _ ?x ?x] ] => rewrite (production_lb (@ascii_lb) eq_refl)
+                 | _ => solve [ trivial ]
+               end.
+        { clear IHls; intros; abstract fin. }
+        { clear IHls; intros; abstract fin. }
+        { clear IHls; intros; abstract fin. }
+        { clear IHls; unfold If_Then_Else, option_rect.
+          repeat match goal with
+                   | [ |- context[if has_only_terminals ?e then _ else _] ]
+                     => case_eq (has_only_terminals e)
+                   | [ |- context[match ?e with None => _ | _ => _ end] ]
+                     => case_eq e
+                 end;
+            try
+              abstract (
+                repeat match goal with
+                         | _ => intro
+                         | _ => progress computes_to_inv
+                         | _ => progress subst
+                         | [ |- In _ [_] ] => left
+                         | [ H : collapse_length_result ?e = Some _ |- _ ]
+                           => (revert H; case_eq e; simpl)
+                         | [ H : Some _ = Some _ |- _ ]
+                           => (inversion H; clear H)
+                         | _ => congruence
+                         | [ H : length_of_any ?G ?nt = same_length ?n,
+                                 p : parse_of_item ?G ?str (NonTerminal ?nt) |- _ ]
+                           => (pose proof (@has_only_terminals_parse_of_item_length G n nt H str p); clear H)
+                         | _ => erewrite <- has_only_terminals_length by eassumption
+                         | _ => progress rewrite ?substring_length, ?Nat.add_sub, ?Nat.sub_0_r, ?Nat.add_0_r, ?minusr_minus
+                         | [ H : _ |- _ ] => generalize dependent H; progress rewrite ?substring_length, ?Nat.add_sub, ?Nat.sub_0_r, ?Nat.add_0_r, ?minusr_minus
+                                                                   | [ H : ?y <= ?x |- context[min ?x ?y] ] => rewrite (Min.min_r x y) by assumption
+                                                                   | [ H : ?x <= ?y |- context[min ?x ?y] ] => rewrite (Min.min_l x y) by assumption
+                                                                   | [ |- context[min ?x (?y + ?z) - ?z] ]
+                                                                     => rewrite <- (Nat.sub_min_distr_r x (y + z) z)
+                                                                   | [ H : context[min ?x (?y + ?z) - ?z] |- _ ]
+                                                                     => generalize dependent H; rewrite <- (Nat.sub_min_distr_r x (y + z) z)
+                                                                                              | [ |- context[min (?x - ?y) ?x] ] => rewrite (Min.min_l (x - y) x) by omega
+                                                                                              | [ |- context[min ?x (?x - ?y)] ] => rewrite (Min.min_r x (x - y)) by omega
+                                                                                              | _ => omega
+                                                                                              | _ => solve [ eauto ]
+                       end
+              ). } } }
+    { intros ???; subst.
+      set (Gnts := Valid_nonterminals G) in * |- .
+      assert (Hvalid : { prefix : _ | List.app prefix Gnts = Valid_nonterminals G }) by (eexists nil; reflexivity).
+      clearbody Gnts.
+      intros.
+      match goal with
+        | [ H : @In string ?nt ?ls |- _ ]
+          => apply (in_map (Lookup G)) in H;
+            generalize dependent (G nt); clear nt; intros
+      end.
+      induction Gnts as [|Gnt Gnts IHG]; [ simpl in *; destruct_head False | ]; [].
+      destruct Hvalid as [prefix Hprefix].
+      simpl in *.
+      repeat match goal with
+               | [ H : context[If productions_beq ?a ?b ?c Then _ Else _] |- _ ]
+                 => destruct (productions_beq a b c) eqn:?; simpl in H
+               | [ H : productions_beq ascii_beq _ _ = true |- _ ]
+                 => apply (productions_bl (@ascii_bl)) in H
+               | [ H : context[productions_beq ascii_beq ?x ?x] |- _ ]
+                 => rewrite (productions_lb (@ascii_lb) (eq_refl x)) in H; simpl in H
+               (*| _ => progress destruct_head' or*)
+               | _ => progress specialize_by assumption
+               | _ => progress specialize_by ltac:(rewrite List.app_assoc; assumption)
+               | _ => progress specialize_by ltac:(rewrite <- List.app_assoc; assumption)
+               | _ => assumption
+               | [ H : ?x = ?y \/ _, H' : productions_beq ascii_beq (?f ?x) (?f ?y) = false |- _ ]
+                 => destruct H
+               | _ => progress subst
+               | [ H : (?prefix ++ ?x :: ?xs = ?ys)%list, H' : { prefix' : _ | (prefix' ++ ?xs = ?ys)%list } -> ?T |- _ ]
+                 => specialize (fun k => H' (existT _ (prefix ++ [x])%list k))
+               | _ => progress cbv beta in *
+               | _ => discriminate
+               | [ H : ?x = ?y \/ _, H' : productions_beq ascii_beq ?x ?y = false |- _ ]
+                 => destruct H
+             end;
+        [].
+      repeat match goal with
+               | [ H : context[match ?x with nil => _ | _ => _ end], H' : List.length ?x = _ |- _ ]
+                 => destruct x eqn:?; simpl in H'
+               | [ H : context[match ?x with nil => _ | _ => _ end] |- _ ]
+                 => destruct (List.length x) eqn:?
+               | [ |- In ?x [?x] ] => left; reflexivity
+               | [ H : context[If productions_beq ?a ?b ?c Then _ Else _] |- _ ]
+                 => destruct (productions_beq a b c) eqn:?; simpl in H
+               | [ H : productions_beq ascii_beq _ _ = true |- _ ]
+                 => apply (productions_bl (@ascii_bl)) in H
+               | [ H : context[productions_beq ascii_beq ?x ?x] |- _ ]
+                 => rewrite (productions_lb (@ascii_lb) (eq_refl x)) in H
+               | _ => progress specialize_by assumption
+               | _ => progress specialize_by ltac:(rewrite List.app_assoc; assumption)
+               | _ => progress specialize_by ltac:(rewrite <- List.app_assoc; assumption)
+               | _ => assumption
+               | [ H : ?x = ?y \/ _, H' : productions_beq ascii_beq (?f ?x) (?f ?y) = false |- _ ]
+                 => destruct H
+               | _ => progress subst
+               | [ H : (?prefix ++ ?x :: ?xs = ?ys)%list, H' : { prefix' : _ | (prefix' ++ ?xs = ?ys)%list } -> ?T |- _ ]
+                 => specialize (fun k => H' (existT _ (prefix ++ [x])%list k))
+               | _ => progress cbv beta in *
+               | _ => progress unfold value in *
+               | [ H : Some ?x = Some ?y |- _ ] => inversion H; clear H
+               | [ H : S ?x = S ?y |- _ ] => inversion H; clear H
+               | _ => progress computes_to_inv
+               | _ => discriminate
+             end;
+        try solve [
               repeat match goal with
-                       | _ => intro
-                       | _ => progress computes_to_inv
+                       | [ |- In ?x [?x] ] => left; reflexivity
+                       | [ H : nil = ?x, H' : context[?x] |- _ ] => progress rewrite <- H in H'
+                       | [ H : (_::_) = ?x, H' : context[?x] |- _ ] => progress rewrite <- H in H'
+                       | [ H : nth_error nil ?n = _ |- _ ] => is_var n; destruct n; simpl in H
+                       | [ H : nth_error (_::_) ?n = _ |- _ ] => is_var n; destruct n; simpl in H
+                       | _ => discriminate
+                     end ].
+      repeat match goal with
+               | [ H : (?x::?xs) = _, H' : context[?x::?xs] |- _ ] => progress rewrite H in H'; try clear H x
+               | [ H : _ = (?x::?xs), H' : context[?x::?xs] |- _ ] => progress rewrite <- H in H'; try clear H x
+               | [ H : ?x = ?x \/ _ |- _ ] => clear H
+             end.
+      clear IHG.
+      generalize dependent its.
+      repeat match goal with
+               | [ H : context[option_rect _ _ _ ?x] |- _ ] => destruct x eqn:?; unfold option_rect in H
+               | [ H : context[If ?e Then _ Else _] |- _ ] => destruct e eqn:?; simpl in H
+             end;
+        try solve [
+              repeat match goal with
+                       | _ => progress intros
+                       | [ |- ?x = ?x \/ _ ] => left; reflexivity
+                       | [ |- In ?x [?x] ] => left; reflexivity
+                       | [ H : nth_error nil ?n = _ |- _ ] => is_var n; destruct n
+                       | [ H : nth_error [_] ?n = _ |- _ ] => is_var n; destruct n as [|[|]]
+                       | [ H : nth_error (_::_) 0 = _ |- _ ] => simpl in H
+                       | [ H : Some _ = Some _ |- _ ] => inversion H; clear H
                        | _ => progress subst
-                       | [ |- In _ [_] ] => left
-                       | [ H : collapse_length_result ?e = Some _ |- _ ]
-                         => (revert H; case_eq e; simpl)
-                       | [ H : Some _ = Some _ |- _ ]
-                         => (inversion H; clear H)
+                       | _ => progress unfold value in *
+                       | _ => discriminate
+                       | [ H : context[option_rect _ _ _ ?x] |- _ ] => destruct x eqn:?; unfold option_rect in H
+                       | _ => progress computes_to_inv
+                       | [ H : context[If ?e Then _ Else _] |- _ ] => destruct e eqn:?; simpl in H
+                       | [ H : StringLike.get _ _ = None |- _ ] => apply no_first_char_empty in H
+                       | [ H' : get 0 ?str = Some _, H : Forall_parse_of_production _ _ |- _ ]
+                         => pose proof ((proj1 (FirstChar.first_char_in_get_str _ _ H'))
+                                          (possible_first_terminals_of_production_correct _ (snd (expand_forall_parse_of_production_default _) H)));
+                           clear H'
+                       | [ H : List.In _ _ |- _ ] => apply (list_in_lb (@ascii_lb)) in H
                        | _ => congruence
-                       | [ H : length_of_any ?G ?nt = same_length ?n,
-                               p : parse_of_item ?G ?str (NonTerminal ?nt) |- _ ]
-                         => (pose proof (@has_only_terminals_parse_of_item_length G n nt H str p); clear H)
-                       | _ => erewrite <- has_only_terminals_length by eassumption
-                       | _ => progress rewrite ?substring_length, ?Nat.add_sub, ?Nat.sub_0_r, ?Nat.add_0_r, ?minusr_minus
-                       | [ H : _ |- _ ] => generalize dependent H; progress rewrite ?substring_length, ?Nat.add_sub, ?Nat.sub_0_r, ?Nat.add_0_r, ?minusr_minus
-                                                                 | [ H : ?y <= ?x |- context[min ?x ?y] ] => rewrite (Min.min_r x y) by assumption
-                                                                 | [ H : ?x <= ?y |- context[min ?x ?y] ] => rewrite (Min.min_l x y) by assumption
-                                                                 | [ |- context[min ?x (?y + ?z) - ?z] ]
-                                                                   => rewrite <- (Nat.sub_min_distr_r x (y + z) z)
-                                                                 | [ H : context[min ?x (?y + ?z) - ?z] |- _ ]
-                                                                   => generalize dependent H; rewrite <- (Nat.sub_min_distr_r x (y + z) z)
-                                                                                            | [ |- context[min (?x - ?y) ?x] ] => rewrite (Min.min_l (x - y) x) by omega
-                                                                                            | [ |- context[min ?x (?x - ?y)] ] => rewrite (Min.min_r x (x - y)) by omega
-                                                                                            | _ => omega
-                                                                                            | _ => solve [ eauto ]
+                       | _ => progress specialize_by assumption
+                       | _ => progress specialize_by ltac:(eapply in_prefix_app; eassumption)
+                       | [ H : forall n a b c d, List.In n ?v |- List.In ?n' ?v ] => specialize (H n')
+                       | _ => progress unfold rules_list_is_complete_case, rules_list_is_complete in *
+                       | [ H : ?G ?x = ?y, H' : forall x', ?G x' = ?y -> ?T |- _ ] => specialize (H' _ H)
+                       | [ H : ?x = (_::_), H' : context[?x] |- _ ] => rewrite H in H'
+                       | [ H : context[nth_error (_::_) 0] |- _ ] => simpl in H
+                       | _ => solve [ eauto with nocore ]
+                       | [ H : forall x, ?f ?y = ?f x -> ?T |- _ ] => specialize (H _ eq_refl)
+                       | [ H : Forall_parse_of_production _ _ |- _ ]
+                         => pose proof (fst (expand_forall_parse_of_production_default _) H); clear H
+                       | _ => simpl; rewrite possible_first_terminals_of_production_empty_correct by eassumption
+                       | _ => left; reflexivity
+                       | [ H : forall x, ?f ?y = ?f x -> ?T |- _ ] => specialize (H _ eq_refl)
+                       | [ H : forall x, ?f x = ?f ?y -> ?T |- _ ] => specialize (H _ eq_refl)
+                       | [ H : forall x, ?k = ?f x -> ?T, H' : ?k = ?f _ |- _ ] => specialize (H _ H')
+                       | [ n : nat |- _ ]
+                         => assert (n = 0)
+                           by (
+                               eapply (@all_disjoint_eq_in _ _ (@ascii_bl)); simpl in *; try eassumption;
+                               match goal with
+                                 | [ |- nth_error (?f (?g ?x) :: map ?f' ?xs) ?n = Some (?f (?g ?y)) ]
+                                   => apply (@map_nth_error _ _ f' n (x::xs) y)
+                               end;
+                               assumption
+                             );
+                           subst
                      end
-            ). } }
+            ].
+      { intros its p Hp H'.
+        assert (n < List.length (G Gnt)).
+        { clear -H'.
+          revert n H'; induction (G Gnt); destruct n; simpl in *; intros; try discriminate; try omega.
+          apply lt_n_S.
+          eauto with nocore. }
+        let H0' := match goal with H0' : computes_to _ _ |- _ => constr:H0' end in
+        apply (all_disjoint_fold_computes_in (n := n)) in H0'; trivial; try first [ exact (@ascii_bl) | exact (@ascii_lb) ];
+        destruct H0' as [[H2 ?]|H2]; subst.
+        { rewrite map_map in H2.
+          repeat match goal with
+                   | [ H' : get 0 ?str = Some _, H : Forall_parse_of_production _ ?p |- _ ]
+                     => pose proof ((proj1 (FirstChar.first_char_in_get_str _ _ H'))
+                                      (possible_first_terminals_of_production_correct _ (snd (expand_forall_parse_of_production_default _) H)));
+                       clear H' H p
+                   | [ H : List.In _ _ |- _ ] => apply (list_in_lb (@ascii_lb)) in H
+                 end.
+          repeat match goal with
+                   | [ H : fold_right orb false _ = false |- _ ] => apply fold_right_orb_false_map_false in H
+                   | [ H : Forall _ _ |- _ ] => rewrite Forall_forall in H
+                   | [ H : context[is_true (negb _)] |- _ ] => setoid_rewrite Bool.negb_true_iff in H
+                   | [ H : nth_error _ _ = Some _ |- _ ] => unique pose proof (nth_error_in H)
+                   | [ H : forall x, ?f x ?y -> ?T, H' : ?f _ ?y |- _ ] => specialize (H _ H')
+                   | _ => congruence
+                 end. }
+        { simpl in *.
+          apply H2; clear H2.
+          exists (possible_first_terminals_of_production G its).
+          repeat match goal with
+                   | [ H' : get 0 ?str = Some _, H : Forall_parse_of_production _ ?p |- _ ]
+                     => pose proof ((proj1 (FirstChar.first_char_in_get_str _ _ H'))
+                                      (possible_first_terminals_of_production_correct _ (snd (expand_forall_parse_of_production_default _) H)));
+                       clear H' H p
+                   | [ H : List.In _ _ |- _ ] => apply (list_in_lb (@ascii_lb)) in H
+                 end.
+          split; [ | assumption ].
+          match goal with
+            | [ |- nth_error (map ?f' ?xs) ?n = Some (?f (?g ?y)) ]
+              => apply (@map_nth_error _ _ f' n xs y)
+          end;
+            assumption. } }
+      { computes_to_inv; subst.
+        intros.
+        (lazymatch goal with
+        | [ |- In ?n (@map ?A ?B ?f (filter ?P ?ls)) ]
+          => apply (@in_map A B f (filter P ls) (n, match nth_error ls n with
+                                                      | None => nil
+                                                      | Some ls' => snd ls'
+                                                    end))
+         end).
+        apply filter_In; simpl.
+        rewrite !nth_error_enumerate; simpl.
+        repeat match goal with
+                 | [ H : ?x = Some _ |- context[?x] ] => rewrite H
+                 | _ => progress simpl
+                 | [ H : StringLike.get _ _ = None |- _ ] => apply no_first_char_empty in H
+                 | [ H' : length _ = 0, H : Forall_parse_of_production _ _ |- _ ]
+                   => pose proof ((possible_first_terminals_of_production_empty_correct H' _ (snd (expand_forall_parse_of_production_default _) H)));
+                     clear H'
+                 | [ H : List.In _ _ |- _ ] => apply (list_in_lb (@ascii_lb)) in H
+                 | [ H : is_true ?b |- context[?b] ] => rewrite H
+                 | [ |- and _ _ ] => split
+                 | [ |- ?x = ?x ] => reflexivity
+               end.
+      apply (nth_error_in_enumerate (k := 0)); assumption. } }
   Qed.
 End IndexedImpl.
