src/Parsers/Splitters/BruteForce.v
@@ -29,34 +29,66 @@ Section brute_force_splitter.
       destruct H; subst; [ right; eauto | left; reflexivity ]. }
   Qed.
 
+  Fixpoint up_to_rev (n : nat) : list nat :=
+    match n with
+      | 0 => nil
+      | S n' => 0::map S (up_to_rev n')
+    end.
+
+  Lemma in_up_to_rev {n m} (H : n < m) : List.In n (up_to_rev m).
+  Proof.
+    revert n H; induction m; intros n H.
+    { exfalso; omega. }
+    { destruct n as [|n].
+      { left; reflexivity. }
+      { right; simpl in *.
+        apply in_map, IHm.
+        omega. } }
+  Qed.
+
   Definition make_all_single_splits (str : String) : list nat
     := (length str)::up_to (length str).
+
+  Definition make_all_production_rules (prods : productions Char) : list nat
+    := up_to_rev (List.length prods).
 
   Context (G : grammar Char).
 
   Global Instance brute_force_data : @boolean_parser_dataT Char _
     := { predata := @rdp_list_predata _ G;
-         split_string_for_production it its := make_all_single_splits }.
+         split_string_for_production it its := make_all_single_splits;
+         select_production_rules prods str := make_all_production_rules prods }.
 
   Global Instance brute_force_cdata : @boolean_parser_completeness_dataT' _ _ G brute_force_data
-    := { split_string_for_production_complete str0 valid str pf it its
-         := ForallT_all (fun _ => Forall_tails_all (fun prod => _)) }.
+    := { split_string_for_production_complete len0 valid str pf it its
+         := ForallT_all (fun _ => Forall_tails_all (fun prod => _));
+         select_production_rules_complete len0 valid str pf nt Hvalid := _ }.
   Proof.
-    destruct prod; try solve [ constructor ].
-    hnf.
-    intros [ n [ p0 p1 ] ].
-    destruct (Compare_dec.le_lt_dec (length str) n).
-    { exists (length str); simpl; repeat split.
-      { left; reflexivity. }
-      { eapply expand_minimal_parse_of_item; [ .. | eassumption ];
-        try solve [ reflexivity
-                  | left; reflexivity
-                  | rewrite !take_long; trivial; reflexivity ]. }
-      { eapply expand_minimal_parse_of_production; [ .. | eassumption ];
-        try solve [ reflexivity
-                  | left; reflexivity
-                  | apply bool_eq_empty; rewrite drop_length; omega ]. } }
-    { exists n; simpl; repeat split; try assumption.
-      right; apply in_up_to; assumption. }
+    { destruct prod; try solve [ constructor ].
+      hnf.
+      intros [ n [ p0 p1 ] ].
+      destruct (Compare_dec.le_lt_dec (length str) n).
+      { exists (length str); simpl; repeat split.
+        { left; reflexivity. }
+        { eapply expand_minimal_parse_of_item; [ .. | eassumption ];
+          try solve [ reflexivity
+                    | left; reflexivity
+                    | rewrite !take_long; trivial; reflexivity ]. }
+        { eapply expand_minimal_parse_of_production; [ .. | eassumption ];
+          try solve [ reflexivity
+                    | left; reflexivity
+                    | apply bool_eq_empty; rewrite drop_length; omega ]. } }
+      { exists n; simpl; repeat split; try assumption.
+        right; apply in_up_to; assumption. } }
+    { hnf.
+      generalize (Lookup G nt); clear.
+      intros prods p.
+      induction p as [ ??? pat pats p | ??? pat pats p [ n [ IHp0 [ pat' IHp1 ] ] ] ].
+      { exists 0; split; [ | exists pat ].
+        { apply in_up_to_rev; simpl; omega. }
+        { split; [ reflexivity | assumption ]. } }
+      { exists (S n); split; [ | exists pat' ].
+        { right; apply in_map; assumption. }
+        { simpl; assumption. } } }
   Qed.
 End brute_force_splitter.
