src/Common/OptionFacts.v
@@ -3,3 +3,9 @@ Lemma option_map_None A B (f : A -> B) x
 Proof.
   destruct x; simpl; split; intros; trivial; congruence.
 Qed.
+
+Lemma option_rect_option_map {A B P} (f : A -> B) (x : option A) a b
+: option_rect P a b (option_map f x) = option_rect (fun k => P (option_map f k)) (fun k => a (f k)) b x.
+Proof.
+  destruct x; simpl; reflexivity.
+Qed.
