src/Parsers/BooleanRecognizer.v
@@ -24,7 +24,8 @@ Section recursive_descent_parser.
       : bool
         := match it with
              | Terminal ch => str ~= [ ch ]
-             | NonTerminal nt => str_matches_nonterminal nt
+             | NonTerminal nt => ((is_valid_nonterminal initial_nonterminals_data nt)
+                                   && str_matches_nonterminal nt)%bool
            end.
 
       Section production.
@@ -75,7 +76,9 @@ Section recursive_descent_parser.
                           (pf : len <= len0),
                      String.string -> bool).
 
-        (** To parse as a given list of [production]s, we must parse as one of the [production]s. *)
+        (** To parse as a given list of [production]s, we must parse
+            as one of the [production]s; we only need to look at the
+            ones labeled by the selection function. *)
         Definition parse_productions'
                    (str : String)
                    (len : nat)
@@ -84,10 +87,11 @@ Section recursive_descent_parser.
         : bool
           := fold_right orb
                         false
-                        (map (parse_production' parse_nonterminal str pf)
-                             prods).
+                        (map (option_rect (fun _ => bool) (fun x => x) false)
+                             (map (option_map (parse_production' parse_nonterminal str pf))
+                                  (map (nth_error prods)
+                                       (select_production_rules prods str)))).
       End productions.
-
 
       Section nonterminals.
         Section step.
@@ -108,35 +112,36 @@ Section recursive_descent_parser.
           : bool.
           Proof.
             refine
-              (parse_productions'
-                 (sumbool_rect
-                    (fun b => forall (str' : String) (len' : nat), len' <= (if b then len else len0) -> String.string -> bool)
-                    (fun _ => (** [str] got smaller, so we reset the valid nonterminals list *)
-                       @parse_nonterminal
-                         (len, nonterminals_length initial_nonterminals_data)
-                         (or_introl _)
-                         initial_nonterminals_data)
-                    (fun _ => (** [str] didn't get smaller, so we cache the fact that we've hit this nonterminal already *)
-                       sumbool_rect
-                         (fun _ => forall (str' : String) (len' : nat), len' <= len0 -> String.string -> bool)
-                         (fun is_valid => (** It was valid, so we can remove it *)
-                            @parse_nonterminal
-                              (len0, pred valid_len)
-                              (or_intror (conj eq_refl _))
-                              (remove_nonterminal valid nt))
+              ((is_valid_nonterminal initial_nonterminals_data nt)
+                 && (parse_productions'
+                       (sumbool_rect
+                          (fun b => forall (str' : String) (len' : nat), len' <= (if b then len else len0) -> String.string -> bool)
+                          (fun _ => (** [str] got smaller, so we reset the valid nonterminals list *)
+                             @parse_nonterminal
+                               (len, nonterminals_length initial_nonterminals_data)
+                               (or_introl _)
+                               initial_nonterminals_data)
+                          (fun _ => (** [str] didn't get smaller, so we cache the fact that we've hit this nonterminal already *)
+                             sumbool_rect
+                               (fun _ => forall (str' : String) (len' : nat), len' <= len0 -> String.string -> bool)
+                               (fun is_valid => (** It was valid, so we can remove it *)
+                                  @parse_nonterminal
+                                    (len0, pred valid_len)
+                                    (or_intror (conj eq_refl _))
+                                    (remove_nonterminal valid nt))
 
-                         (fun _ _ _ _ _ => (** oops, we already saw this nonterminal in the past.  ABORT! *)
-                            false)
-                         (Sumbool.sumbool_of_bool (negb (EqNat.beq_nat valid_len 0) && is_valid_nonterminal valid nt)))
-                    (lt_dec len len0))
-                 str
-                 (len := len)
-                 (sumbool_rect
-                    (fun b => len <= (if b then len else len0))
-                    (fun _ => le_n _)
-                    (fun _ => _)
-                    (lt_dec len len0))
-                 (Lookup G nt));
+                               (fun _ _ _ _ _ => (** oops, we already saw this nonterminal in the past.  ABORT! *)
+                                  false)
+                               (Sumbool.sumbool_of_bool (negb (EqNat.beq_nat valid_len 0) && is_valid_nonterminal valid nt)))
+                          (lt_dec len len0))
+                       str
+                       (len := len)
+                       (sumbool_rect
+                          (fun b => len <= (if b then len else len0))
+                          (fun _ => le_n _)
+                          (fun _ => _)
+                          (lt_dec len len0))
+                       (Lookup G nt)))%bool;
             first [ assumption
                   | simpl;
                     generalize (proj1 (proj1 (Bool.andb_true_iff _ _) is_valid));
