src/Parsers/ContextFreeGrammarPropertiesRDPList.v
@@ -1,0 +1,57 @@
+(** * Properties about Context Free Grammars *)
+Require Import Fiat.Parsers.StringLike.Core Fiat.Parsers.ContextFreeGrammar.
+Require Import Fiat.Parsers.ContextFreeGrammarProperties.
+Require Import Fiat.Parsers.BaseTypes.
+Require Import Fiat.Parsers.Splitters.RDPList.
+Require Import Fiat.Common.
+Require Import Fiat.Common.Equality.
+
+Set Implicit Arguments.
+
+Section convenience.
+  Context {Char} {HSL : StringLike Char} {HSLP : @StringLikeProperties Char HSL}
+          (G : grammar Char).
+
+  Let predata := rdp_list_predata (G := G).
+  Local Existing Instance predata.
+
+  Local Notation iffT A B := ((A -> B) * (B -> A))%type.
+  Local Infix "<->" := iffT : type_scope.
+
+  Local Ltac t Forall_parse_of expand_forall_parse_of parse_of_respectful parse_of_respectful_refl :=
+    repeat match goal with
+             | [ |- context G[@Forall_parse_of _ _ _ ?f _ _ ?p] ]
+               => is_var p;
+                 replace (@Forall_parse_of _ _ _ f _ _ p) with (@Forall_parse_of _ _ _ f _ _ (@parse_of_respectful _ _ _ _ _ _ (reflexivity _) _ p))
+                    by (rewrite parse_of_respectful_refl; reflexivity)
+             | [ |- prod _ _ ] => split
+             | [ |- _ -> _ ] => eapply expand_forall_parse_of
+             | _ => progress simpl
+             | _ => progress unfold rdp_list_is_valid_nonterminal
+             | _ => progress intros
+             | [ H : is_true (list_bin string_beq _ _) |- _ ] => apply (list_in_bl (@string_bl)) in H
+             | [ |- is_true (list_bin string_beq _ _) ] => apply (list_in_lb (@string_lb))
+             | _ => assumption
+           end.
+
+  Definition expand_forall_parse_of_default {str pats} (p : parse_of G str pats)
+  : Forall_parse_of (fun _ nt => is_valid_nonterminal initial_nonterminals_data nt) p
+    <-> Forall_parse_of (fun _ nt => List.In nt (Valid_nonterminals G)) p.
+  Proof.
+    t (@Forall_parse_of) (@expand_forall_parse_of) (@parse_of_respectful) (@parse_of_respectful_refl).
+  Qed.
+
+  Definition expand_forall_parse_of_item_default {str x} (p : parse_of_item G str x)
+  : Forall_parse_of_item (fun _ nt => is_valid_nonterminal initial_nonterminals_data nt) p
+    <-> Forall_parse_of_item (fun _ nt => List.In nt (Valid_nonterminals G)) p.
+  Proof.
+    t (@Forall_parse_of_item) (@expand_forall_parse_of_item) (@parse_of_item_respectful) (@parse_of_item_respectful_refl).
+  Qed.
+
+  Definition expand_forall_parse_of_production_default {str x} (p : parse_of_production G str x)
+  : Forall_parse_of_production (fun _ nt => is_valid_nonterminal initial_nonterminals_data nt) p
+    <-> Forall_parse_of_production (fun _ nt => List.In nt (Valid_nonterminals G)) p.
+  Proof.
+    t (@Forall_parse_of_production) (@expand_forall_parse_of_production) (@parse_of_production_respectful) (@parse_of_production_respectful_refl).
+  Qed.
+End convenience.
