src/Parsers/CorrectnessBaseTypes.v
@@ -24,6 +24,19 @@ Section general.
                    * (minimal_parse_of_item (G := G) len0 valid (take n str) it)
                    * (minimal_parse_of_production (G := G) len0 valid (drop n str) its) }%type).
 
+  Definition select_list_completeT {data : @parser_computational_predataT}
+             {len0 valid}
+             (str : String)
+             (pf : length str <= len0)
+             (prods : productions Char)
+             (select_list : list nat)
+    := minimal_parse_of (G := G) (predata := data) len0 valid str prods
+       -> ({ n : nat
+                   & (In n select_list)
+                     * { its : production Char
+                               & (nth_error prods n = Some its)
+                                 * (minimal_parse_of_production (G := G) len0 valid str its) } })%type.
+
   Class boolean_parser_completeness_dataT' {data : boolean_parser_dataT} :=
     { split_string_for_production_complete
       : forall len0 valid str (pf : length str <= len0) nt,
@@ -36,7 +49,11 @@ Section general.
                         | it::its
                           => @split_list_completeT data len0 valid it its str pf (split_string_for_production it its str)
                       end))
-               (Lookup G nt) }.
+               (Lookup G nt);
+      select_production_rules_complete
+      : forall len0 valid str (pf : length str <= len0) nt,
+          is_valid_nonterminal initial_nonterminals_data nt
+          -> @select_list_completeT data len0 valid str pf (Lookup G nt) (select_production_rules (Lookup G nt) str) }.
 
   Class boolean_parser_correctness_dataT :=
     { data :> boolean_parser_dataT;
