src/Parsers/Refinement/DisjointRules.v
@@ -26,7 +26,6 @@ Definition search_for_condition (G : grammar Ascii.ascii) str its (n : nat)
        (fun ch => list_bin ascii_beq ch (possible_first_terminals_of_production G its)).
 
 Lemma refine_disjoint_search_for' {G : grammar Ascii.ascii}
-      (Hvalid : grammar_rvalid G)
       {str nt its}
       (H_disjoint : disjoint ascii_beq
                              (possible_terminals_of G nt)
@@ -47,7 +46,7 @@ Proof.
   apply PickComputes.
   intros n ? H_reachable pit pits Hpit Hpits.
   left.
-  pose proof (terminals_disjoint_search_for Hvalid _ H_disjoint _ _ H_reachable Hpit Hpits) as H'.
+  pose proof (terminals_disjoint_search_for _ H_disjoint _ _ H_reachable Hpit Hpits) as H'.
   specialize (H1 (ex_intro _ n H')).
   pose proof (is_first_char_such_that_eq_nat_iff H1 H') as H''.
   destruct_head or; destruct_head and; subst; omega.
@@ -61,7 +60,6 @@ Definition search_for_not_condition (G : grammar Ascii.ascii) str nt its n
        (fun ch => negb (list_bin ascii_beq ch (possible_terminals_of G nt))).
 
 Lemma refine_disjoint_search_for_not' {G : grammar Ascii.ascii}
-      (Hvalid : grammar_rvalid G)
       {str nt its}
       (H_disjoint : disjoint ascii_beq
                              (possible_terminals_of G nt)
@@ -82,7 +80,7 @@ Proof.
   apply PickComputes.
   intros n ? H_reachable pit pits Hpit Hpits.
   left.
-  pose proof (terminals_disjoint_search_for_not Hvalid _ H_disjoint _ _ H_reachable Hpit Hpits) as H'.
+  pose proof (terminals_disjoint_search_for_not _ H_disjoint _ _ H_reachable Hpit Hpits) as H'.
   specialize (H1 (ex_intro _ n H')).
   pose proof (is_first_char_such_that_eq_nat_iff H1 H') as H''.
   destruct_head or; destruct_head and; subst; omega.
@@ -181,7 +179,6 @@ Proof.
 Qed.
 
 Lemma refine_disjoint_search_for {G : grammar Ascii.ascii} {str nt its}
-      (Hvalid : grammar_rvalid G)
       (H_disjoint : disjoint ascii_beq
                              (possible_terminals_of G nt)
                              (possible_first_terminals_of_production G its))
@@ -198,7 +195,6 @@ Proof.
 Qed.
 
 Lemma refine_disjoint_search_for_not {G : grammar Ascii.ascii} {str nt its}
-      (Hvalid : grammar_rvalid G)
       (H_disjoint : disjoint ascii_beq
                              (possible_terminals_of G nt)
                              (possible_first_terminals_of_production G its))
